changes use of variable l for effect operations to op; changes notation of handlers

theories/case_studies/promptcontrol.v
@@ -25,46 +25,45 @@ From haffel.logic Require Import sem_operators.
 From haffel.logic Require Import compatibility.
 From haffel.logic Require Import tactics.
 
-Definition deep_try_alt_ls : val := (
-  rec: "H" "e" "l" "h" "r" :=
-    shallow_try_ls "e" "l" (λ: "x" "k", "H" (λ: <>, "h" "x" "k") "l" "h" "r") "r"
+Definition handler_alt : val := (
+  rec: "H" "e" "op" "h" "r" :=
+    shandler "e" "op" (λ: "x" "k", "H" (λ: <>, "h" "x" "k") "op" "h" "r") "r"
 )%V.
 
-Arguments deep_try_alt_ls : simpl never.
+Arguments handler_alt : simpl never.
 
-Definition DeepTryAltLS (e : expr) (l : label) (h r : expr) : expr :=
-  deep_try_alt_ls (λ: <>, e)%E (effect l)%V h r.
+Definition HandlerAlt (e : expr) (op : operation) (h r : expr) : expr :=
+  handler_alt (λ: <>, e)%E (effect op) h r.
 
-Definition DeepTryAltLSV (e : expr) (l : label) (h r : expr) : expr :=
-  deep_try_alt_ls (λ: <>, e)%V (effect l)%V h r.
+Definition HandlerAltV (e : expr) (op : operation) (h r : expr) : expr :=
+  handler_alt (λ: <>, e)%V (effect op) h r.
 
-Notation "'deep-try-alt-ls:' e 'handle' l 'with' 'effect' h | 'return' r 'end'" :=
-  (DeepTryAltLS e l h r)
-  (e, l, h, r at level 200, only parsing) : expr_scope.
+Notation "'handle-alt:' e 'by' op '=>' h | 'ret' => r 'end'" :=
+  (HandlerAlt e op h r)
+  (e, op, h, r at level 200, only parsing) : expr_scope.
 
-Definition control : val := (Λ: Λ: λ: "f", perform: (effect "ctrl", "f"))%V.
-Definition controlₘ : val := (Λ: Λ: λ: "f", performₘ: (effect "ctrl", "f"))%V.
+Definition control : val := (Λ: Λ: λ: "f", perform: "ctrl" "f")%V.
+Definition controlₘ : val := (Λ: Λ: λ: "f", performₘ: "ctrl" "f")%V.
 
 Definition prompt : val := 
   (Λ: λ: "e", 
-    deep-try-alt-ls: "e" #() handle "ctrl" with 
-                effect (λ: "x" "k", "x" "k")
-              | return (λ: "x", "x")
-             end
-  )%V.
+    handle-alt: "e" #() by 
+      "ctrl" => (λ: "x" "k", "x" "k")
+    |  ret   => (λ: "x", "x")
+    end)%V.
 
-Section deep_handler_alt.
+Section handler_alt.
 
   Context `{!heapGS Σ}.
   
-  Notation deep_handler_alt_ls_type Σ :=
-    (coPset -d> label-d> sem_sig Σ -d> sem_row Σ -d> mode -d> (val -d> iPropO Σ) 
+  Notation handler_alt_spec_type Σ :=
+    (coPset -d> operation-d> sem_sig Σ -d> sem_row Σ -d> mode -d> (val -d> iPropO Σ) 
             -d> expr -d> expr
             -d> sem_row Σ -d> (val -d> iPropO Σ) -d> iPropO Σ) (only parsing).
   
     (* Correctness of the effect branch. *)
-  Definition deep_handler_alt_ls `{irisGS eff_lang Σ} : deep_handler_alt_ls_type Σ := (
-    λ E l σ ρ m Φ h r ρ' Φ',
+  Definition handler_alt_spec `{irisGS eff_lang Σ} : handler_alt_spec_type Σ := (
+    λ E op σ ρ m Φ h r ρ' Φ',
     
     (* Subsumption on row *)
     (ρ ≤R ρ') ∗
@@ -80,49 +79,49 @@ Section deep_handler_alt.
     (* Correctness of the effect branch. *)
     □ (
       ∀ (v k : val),
-        iEff_car (upcl σ.1 σ.2) v (λ w, EWPW k w @ E <| (l, σ) ·: ρ |> {{ Φ }}) -∗
-        EWPW h v k @ E <| (l, σ) ·: ρ |> {{ Φ }}
+        iEff_car (upcl σ.1 σ.2) v (λ w, EWPW k w @ E <| (op, σ) ·: ρ |> {{ Φ }}) -∗
+        EWPW h v k @ E <| (op, σ) ·: ρ |> {{ Φ }}
     ))%I.
   
-  Lemma ewpw_deep_try_alt_ls E (l : label) m σ ρ ρ' e (h r : val) Φ Φ' :
-    EWPW e @ E <| (l, σ) ·: ρ |> {{ Φ }} -∗
-    deep_handler_alt_ls E l σ ρ m Φ h r ρ' Φ' -∗
-    EWPW (DeepTryAltLSV e l h r) @E <| ρ' |> {{ Φ' }}.
+  Lemma ewpw_handler_alt E (op : operation) m σ ρ ρ' e (h r : val) Φ Φ' :
+    EWPW e @ E <| (op, σ) ·: ρ |> {{ Φ }} -∗
+    handler_alt_spec E op σ ρ m Φ h r ρ' Φ' -∗
+    EWPW (HandlerAltV e op h r) @E <| ρ' |> {{ Φ' }}.
   Proof.
-    iIntros "He H". rewrite /DeepTryAltLSV. 
-    iLöb as "IH" forall (e). rewrite /deep_try_alt_ls /ewpw. 
-    rewrite /deep_handler_alt_ls.
+    iIntros "He H". rewrite /HandlerAltV. 
+    iLöb as "IH" forall (e). rewrite /handler_alt /ewpw. 
+    rewrite /handler_alt_spec.
     do 10 ewp_value_or_step. ewp_pure_steps. 
-    iApply (ewpw_shallow_try_ls _ l m  with "He").
+    iApply (ewpw_shandler _ op m  with "He").
     iDestruct "H" as "(#H1 & %H2 & H3 & #H4)".
-    rewrite /shallow_handler_ls. iFrame "#%".
+    rewrite /shandler. iFrame "#%".
     destruct m; simpl.
     - iSplit; first iApply "H3".
       iIntros (v k) "(%Φ'' & Hσ & HPost)".
       rewrite /ewpw; do 6 ewp_value_or_step. 
-      rewrite -/deep_try_alt_ls. iApply ("IH" with "[Hσ HPost]").
+      rewrite -/handler_alt. iApply ("IH" with "[Hσ HPost]").
       { iApply "H4". iExists Φ''. iFrame. }
       iFrame "#%∗".
     - iDestruct "H3" as "#H3". iIntros "!#".
       iFrame "#". iIntros (v k) "(%Φ'' & Hσ & HPost)".
       rewrite /ewpw; do 6 ewp_value_or_step. 
-      rewrite -/deep_try_alt_ls. iApply ("IH" with "[Hσ HPost]").
+      rewrite -/handler_alt. iApply ("IH" with "[Hσ HPost]").
       { iApply "H4". iExists Φ''. iFrame. }
       iFrame "#%∗".
   Qed.
   
-  Lemma sem_typed_deep_try_alt_os m l A B τ τ' ρ' ρ'' Γ₁ Γ₂ Γ₃ Γ' x k e h r `{NonExpansive A, NonExpansive B}:
+  Lemma sem_typed_handler_alt_os m op A B τ τ' ρ' ρ'' Γ₁ Γ₂ Γ₃ Γ' x k e h r `{NonExpansive A, NonExpansive B}:
       x ∉ env_dom Γ₂ → x ∉ env_dom Γ' → x ∉ env_dom Γ₃ → x ∉ env_dom Γ₂ → k ∉ env_dom Γ₂ → k ∉ env_dom Γ₃ → k ∉ env_dom Γ' → x ≠ k →
       let σ := (∀S: α, A α ⇒ B α | m)%S in
-      let ρ := ((l, σ) ·: ρ')%R in
+      let ρ := ((op, σ) ·: ρ')%R in
       copy_env Γ' -∗
       ρ' ≤R ρ'' -∗
       Γ₁ ⊨ e : ρ : τ ⊨ Γ₂ -∗
       (∀ α, (x, A α) :: (k, B α -{ ρ }-∘ τ) :: Γ' ⊨ h : ρ : τ ⊨ Γ₂) -∗
       (x, τ) :: Γ₂ ++ Γ' ⊨ r : ρ'' : τ' ⊨ Γ₃ -∗
-      Γ₁ ++ Γ' ⊨ (deep-try-alt-ls: e handle l with
-                          effect  (λ: x k, h)
-                        | return  (λ: x, r) end)%E : ρ'' : τ' ⊨ Γ₃.
+      Γ₁ ++ Γ' ⊨ (handle-alt: e by 
+                     op => (λ: x k, h)
+                  | ret => (λ: x, r) end)%E : ρ'' : τ' ⊨ Γ₃.
     Proof.
       iIntros (??????????) "#Hcpy #Hle #He #Hh #Hr !# %vs HΓ₁Γ' /=".
       iDestruct (env_sem_typed_app with "HΓ₁Γ'") as "[HΓ₁ HΓ'']". 
@@ -131,8 +130,8 @@ Section deep_handler_alt.
       iSpecialize ("He" $! vs with "HΓ₁").
       iRevert "He". iLöb as "IH" forall (e). iIntros "He".
       ewpw_pure_steps. 
-      iApply (ewpw_deep_try_alt_ls _ _ MS with "He [HΓ']").
-      rewrite /deep_handler_alt_ls.
+      iApply (ewpw_handler_alt _ _ MS with "He [HΓ']").
+      rewrite /handler_alt.
       repeat iSplit; eauto. simpl. iIntros "!#". 
       - iIntros (v) "[Hτ HΓ₂]". ewpw_pure_steps. rewrite - subst_map_insert. 
         iApply (ewpw_mono with "[HΓ₂ HΓ' Hτ]").
@@ -153,18 +152,18 @@ Section deep_handler_alt.
         + iIntros "!# /= % [$ H] !>". do 2 (rewrite - env_sem_typed_insert //).
     Qed.
   
-  Lemma sem_typed_deep_try_alt_ms l A B τ τ' ρ' ρ'' Γ₁ Γ₂ Γ₃ Γ' x k e h r `{NonExpansive A, NonExpansive B}:
+  Lemma sem_typed_handler_alt_ms op A B τ τ' ρ' ρ'' Γ₁ Γ₂ Γ₃ Γ' x k e h r `{NonExpansive A, NonExpansive B}:
       x ∉ env_dom Γ₂ → x ∉ env_dom Γ' → x ∉ env_dom Γ₃ → x ∉ env_dom Γ₂ → k ∉ env_dom Γ₂ → k ∉ env_dom Γ₃ → k ∉ env_dom Γ' → x ≠ k →
       let σ := (∀S: α, A α ⇒ B α | MS)%S in
-      let ρ := ((l, σ) ·: ρ')%R in
+      let ρ := ((op, σ) ·: ρ')%R in
       copy_env Γ' -∗
       ρ' ≤R ρ'' -∗
       Γ₁ ⊨ e : ρ : τ ⊨ Γ₂ -∗
       (∀ α, (x, A α) :: (k, B α -{ ρ }-> τ) :: Γ' ⊨ h : ρ : τ ⊨ Γ₂) -∗
       (x, τ) :: Γ₂ ++ Γ' ⊨ r : ρ'' : τ' ⊨ Γ₃ -∗
-      Γ₁ ++ Γ' ⊨ (deep-try-alt-ls: e handle l with
-                          effect  (λ: x k, h)
-                        | return  (λ: x, r) end)%E : ρ'' : τ' ⊨ Γ₃.
+      Γ₁ ++ Γ' ⊨ (handle-alt: e by
+                     op  => (λ: x k, h)
+                   | ret => (λ: x, r) end)%E : ρ'' : τ' ⊨ Γ₃.
     Proof.
       iIntros (??????????) "#Hcpy #Hle #He #Hh #Hr !# %vs HΓ₁Γ' /=".
       iDestruct (env_sem_typed_app with "HΓ₁Γ'") as "[HΓ₁ HΓ'']". 
@@ -173,8 +172,8 @@ Section deep_handler_alt.
       iSpecialize ("He" $! vs with "HΓ₁").
       iRevert "He". iLöb as "IH" forall (e). iIntros "He".
       ewpw_pure_steps. 
-      iApply (ewpw_deep_try_alt_ls _ _ MS with "He [HΓ']").
-      rewrite /deep_handler_alt_ls.
+      iApply (ewpw_handler_alt _ _ MS with "He [HΓ']").
+      rewrite /handler_alt.
       repeat iSplit; eauto. simpl. iIntros "!#". 
       - iIntros (v) "[Hτ HΓ₂]". ewpw_pure_steps. rewrite - subst_map_insert. 
         iApply (ewpw_mono with "[HΓ₂ HΓ' Hτ]").
@@ -194,13 +193,13 @@ Section deep_handler_alt.
         + iIntros "!# /= % [$ H] !>". do 2 (rewrite - env_sem_typed_insert //).
     Qed.
 
-End deep_handler_alt.
+End handler_alt.
 
 Section typing.
 
   Context `{!heapGS Σ}.
 
-  Definition ctrl_sig (β : sem_ty Σ) (ctrl : sem_row Σ) : label * sem_sig Σ := 
+  Definition ctrl_sig (β : sem_ty Σ) (ctrl : sem_row Σ) : operation * sem_sig Σ := 
       ("ctrl", ∀S: α , (α -{ ctrl }-∘ β) -{ ctrl }-∘ β ⇒ α | OS)%S.
 
   Definition ctrl_pre (β : sem_ty Σ) (ctrl : sem_row Σ) : sem_row Σ := 
@@ -260,7 +259,7 @@ Section typing.
     iApply sem_typed_ufun; solve_sidecond. simpl.
     rewrite - (app_nil_r [("e", _)]).
     set Γ₁ := [("e", () -{ ctrl β }-∘ β)].
-    iApply (sem_typed_deep_try_alt_os OS "ctrl" (λ α, (α -{ ctrl β }-∘ β) -{ ctrl β }-∘ β) (λ α,  α) β β ⟨⟩%R ⟨⟩%R Γ₁ [] [] []); solve_sidecond.  
+    iApply (sem_typed_handler_alt_os OS "ctrl" (λ α, (α -{ ctrl β }-∘ β) -{ ctrl β }-∘ β) (λ α,  α) β β ⟨⟩%R ⟨⟩%R Γ₁ [] [] []); solve_sidecond.  
     { iApply row_le_nil. }
     - rewrite /Γ₁. iApply sem_typed_sub_row. 
       { iApply (row_le_rec_unfold (λ θ, ctrl_pre β θ)). }
