theories/logic/ewpw.v
@@ -282,18 +282,18 @@ Proof.
   by iApply ewp_eff_os.
 Qed.
 
-Lemma ewpw_do_os E l s v ρ Φ :
-  iEff_car ⟦ filter_os ρ ⟧%R ((effect l, s), v)%V Φ -∗ 
-  EWPW (do: ((effect l, s), v)%V) @ E <| ρ |> {{ Φ }}.
+Lemma ewpw_do_os E op s v ρ Φ :
+  iEff_car ⟦ filter_os ρ ⟧%R (effect op, s, v)%V Φ -∗ 
+  EWPW (do: (effect op, s, v)%V) @ E <| ρ |> {{ Φ }}.
 Proof.
   iIntros "Hρ".
   rewrite /ewpw /=. iApply ewp_do_os.
   simpl. iExists Φ. iFrame. iIntros (w) "$".
 Qed.
 
-Lemma ewpw_do_ms E l s v ρ Φ :
-  iEff_car ⟦ ρ ⟧%R ((effect l, s), v)%V Φ -∗ 
-  EWPW (doₘ: ((effect l, s), v)%V) @ E <| ρ |> {{ Φ }}.
+Lemma ewpw_do_ms E op s v ρ Φ :
+  iEff_car ⟦ ρ ⟧%R (effect op, s, v)%V Φ -∗ 
+  EWPW (doₘ: (effect op, s, v)%V) @ E <| ρ |> {{ Φ }}.
 Proof.
   iIntros "Hρ".
   rewrite /ewpw /=. 
@@ -301,9 +301,9 @@ Proof.
   simpl; iExists Φ; iFrame; iIntros "!# % $".
 Qed.
 
-Lemma ewpw_lft E l σ ρ e Φ :
+Lemma ewpw_lft E op σ ρ e Φ :
   EWPW e @E  <| ρ |> {{ Φ }} -∗
-  EWPW (lft: (effect l, e)) @E <| (l, σ) ·: ρ |> {{ Φ }}.
+  EWPW (lft: op e) @E <| (op, σ) ·: ρ |> {{ Φ }}.
 Proof. 
   iIntros "He".
   rewrite /lft_def. rewrite /ewpw. ewp_pure_steps.
@@ -314,44 +314,44 @@ Proof.
   iSplit; last iSplit.
   - iIntros (v) "HΦ". by ewp_pure_steps.
   - iIntros (v k) "Hρ".
-    iDestruct "Hρ" as "(%Φ' & (%w & %l' & %s' & %σ' & -> & #Hlookup' & Hσ') & HPost)". 
+    iDestruct "Hρ" as "(%Φ' & (%w & %op' & %s' & %σ' & -> & #Hlookup' & Hσ') & HPost)". 
     ewp_pure_steps'.
-    destruct (decide (l = l')) as [->|Hneg].
+    destruct (decide (op = op')) as [->|Hneg].
     + ewp_pure_steps'. iApply ewp_do_os. 
       rewrite filter_os_lookup. iExists Φ'. simpl.
       iSplitL "Hσ'".
-      { iExists w, l', (S s'), σ'. rewrite /sem_row_cons. 
+      { iExists w, op', (S s'), σ'. rewrite /sem_row_cons. 
         rewrite filter_os_lookup /sem_row_ins lookup_insert_ne // row_tun_lookup_alt. iFrame "#∗". 
         by replace (Z.add (Z.of_nat s') (Zpos xH)) with (Z.of_nat (S s')) by lia. }
       iIntros (v') "HΦ'". iApply ("HPost" with "HΦ'"). by iNext.
     + ewp_pure_steps'. iApply ewp_do_os. 
       rewrite filter_os_lookup. iExists Φ'. simpl.
       iSplitL "Hσ'".
-      { iExists w, l', s', σ'. 
+      { iExists w, op', s', σ'. 
         rewrite filter_os_lookup /sem_row_cons /sem_row_ins lookup_insert_ne //; last (intros H; inv H).
         rewrite row_tun_lookup_ne //. by iFrame "#∗".  }
       iIntros (v') "HΦ'". iApply ("HPost" with "HΦ'"). by iNext.
   - iIntros (v k) "Hρ". simpl.
-    iDestruct "Hρ" as "(%Φ' & (%w & %l' & %s' & %σ' & -> & #Hlookup' & Hσ') & #HPost)". 
+    iDestruct "Hρ" as "(%Φ' & (%w & %op' & %s' & %σ' & -> & #Hlookup' & Hσ') & #HPost)". 
     ewp_pure_steps'.
-    destruct (decide (l = l')) as [->|Hneg].
+    destruct (decide (op = op')) as [->|Hneg].
     + ewp_pure_steps'. iApply ewp_do_ms. 
       iExists Φ'. simpl.
       iSplitL "Hσ'".
-      { iExists w, l', (S s'), σ'. rewrite /sem_row_cons /sem_row_ins lookup_insert_ne // row_tun_lookup_alt. iFrame "#∗". 
+      { iExists w, op', (S s'), σ'. rewrite /sem_row_cons /sem_row_ins lookup_insert_ne // row_tun_lookup_alt. iFrame "#∗". 
         by replace (Z.add (Z.of_nat s') (Zpos xH)) with (Z.of_nat (S s')) by lia. }
       iIntros "!# %v' HΦ'". iApply ("HPost" with "HΦ'"). by iNext.
     + ewp_pure_steps'. iApply ewp_do_ms. iExists Φ'. simpl.
       iSplitL "Hσ'".
-      { iExists w, l', s', σ'. 
+      { iExists w, op', s', σ'. 
         rewrite /sem_row_cons /sem_row_ins lookup_insert_ne; last (intros H; inv H). 
         rewrite row_tun_lookup_ne //. by iFrame "#∗".  }
       iIntros "!# %v' HΦ'". iApply ("HPost" with "HΦ'"). by iNext.
 Qed.
 
-Lemma ewpw_unlft E l ρ e Φ :
-  EWPW e @E <| ⦗ ρ | l ⦘ |> {{ Φ }} -∗
-  EWPW (unlft: (effect l, e)) @E <| ρ |> {{ Φ }}.
+Lemma ewpw_unlft E op ρ e Φ :
+  EWPW e @E <| ⦗ ρ | op ⦘ |> {{ Φ }} -∗
+  EWPW (unlft: op e) @E <| ρ |> {{ Φ }}.
 Proof.
   iIntros "He".
   rewrite /unlft_def. rewrite /ewpw. ewp_pure_steps.
@@ -362,51 +362,51 @@ Proof.
   iSplit; last iSplit.
   - iIntros (v) "HΦ". by ewp_pure_steps.
   - iIntros (v k) "Hρ".
-    iDestruct "Hρ" as "(%Φ' & (%w & %l' & %s' & %σ' & -> & #Hlookup' & Hσ') & HPost)". 
+    iDestruct "Hρ" as "(%Φ' & (%w & %op' & %s' & %σ' & -> & #Hlookup' & Hσ') & HPost)". 
     ewp_pure_steps'.
-    destruct (decide (l = l')) as [->|Hneg].
+    destruct (decide (op = op')) as [->|Hneg].
     + ewp_pure_steps'. iApply ewp_do_os. 
       rewrite filter_os_lookup row_tun_lookup. 
       iDestruct "Hlookup'" as "[(%s & -> & Hlookup) HOS]". iExists Φ'. simpl.
       iSplitL "Hσ'".
-      { iExists w, l', s, σ'. rewrite filter_os_lookup. iFrame "#∗". 
+      { iExists w, op', s, σ'. rewrite filter_os_lookup. iFrame "#∗". 
         by replace (Z.sub (Z.of_nat (S s)) (Zpos xH)) with (Z.of_nat s) by lia. }
       iIntros (v') "HΦ'". iApply ("HPost" with "HΦ'"). by iNext.
     + ewp_pure_steps'. iApply ewp_do_os. 
       rewrite filter_os_lookup row_tun_lookup_ne //. iExists Φ'. simpl.
       iSplitL "Hσ'".
-      { iExists w, l', s', σ'. rewrite filter_os_lookup //. by iFrame "#∗".  }
+      { iExists w, op', s', σ'. rewrite filter_os_lookup //. by iFrame "#∗".  }
       iIntros (v') "HΦ'". iApply ("HPost" with "HΦ'"). by iNext.
   - iIntros (v k) "Hρ". simpl.
-    iDestruct "Hρ" as "(%Φ' & (%w & %l' & %s' & %σ' & -> & #Hlookup' & Hσ') & #HPost)". 
+    iDestruct "Hρ" as "(%Φ' & (%w & %op' & %s' & %σ' & -> & #Hlookup' & Hσ') & #HPost)". 
     ewp_pure_steps'.
-    destruct (decide (l = l')) as [->|Hneg].
+    destruct (decide (op = op')) as [->|Hneg].
     + ewp_pure_steps'. iApply ewp_do_ms. 
       rewrite row_tun_lookup. iDestruct "Hlookup'" as "(%s & -> & Hlookup)". 
       iExists Φ'. simpl.
       iSplitL "Hσ'".
-      { iExists w, l', s, σ'. iFrame "#∗". 
+      { iExists w, op', s, σ'. iFrame "#∗". 
         by replace (Z.sub (Z.of_nat (S s)) (Zpos xH)) with (Z.of_nat s) by lia. }
       iIntros "!# %v' HΦ'". iApply ("HPost" with "HΦ'"). by iNext.
     + ewp_pure_steps'. iApply ewp_do_ms. iExists Φ'. simpl.
       iSplitL "Hσ'".
-      { iExists w, l', s', σ'. rewrite row_tun_lookup_ne //. by iFrame "#∗".  }
+      { iExists w, op', s', σ'. rewrite row_tun_lookup_ne //. by iFrame "#∗".  }
       iIntros "!# %v' HΦ'". iApply ("HPost" with "HΦ'"). by iNext.
 Qed.
 
-Lemma handler_effect_propagated_cond E l l' s' Ψ :
- ¬ (l = l' ∧ s' = 0) →
- ⊢ EWP if: (effect l')%V = (effect l)%V then #s' = #0 else #false @ E <| Ψ |> {{ v, ⌜v = #false⌝ }}.
+Lemma handler_effect_propagated_cond E op op' s' Ψ :
+ ¬ (op = op' ∧ s' = 0) →
+ ⊢ EWP if: (effect op') = (effect op)%V then #s' = #0 else #false @ E <| Ψ |> {{ v, ⌜v = #false⌝ }}.
 Proof.
   intros Hneg. rewrite not_and_l in Hneg. iIntros.
-  destruct (decide (l = l')) as [->|], Hneg; ewp_pure_steps'. 
+  destruct (decide (op = op')) as [->|], Hneg; ewp_pure_steps'. 
   iPureIntro. rewrite bool_decide_false //. 
   intros H'. simplify_eq. assert (s' = 0) by lia. simplify_eq. 
 Qed.
 
-Definition shallow_handler_ls
+Definition shandler_spec
   (E : coPset)
-  (l : label)
+  (op : operation)
   (σ : sem_sig Σ)
   (ρ : sem_row Σ)
   (m : mode)
@@ -426,26 +426,26 @@ Definition shallow_handler_ls
 
   (* Correctness of the effect branch. *)
   (∀ (v k : val),
-     iEff_car (upcl σ.1 σ.2) v (λ w, EWPW k w @ E <| (l, σ) ·: ρ |> {{ Φ }}) -∗
+     iEff_car (upcl σ.1 σ.2) v (λ w, EWPW k w @ E <| (op, σ) ·: ρ |> {{ Φ }}) -∗
        EWPW h v k @ E <| ρ' |> {{ Φ' }}))
   )%I.
 
-Lemma ewpw_shallow_try_ls E (l : label) m σ ρ ρ' e (h r : val) Φ Φ' :
-  EWPW e @ E <| (l, σ) ·: ρ |> {{ Φ }} -∗
-  shallow_handler_ls E l σ ρ m Φ h r ρ' Φ' -∗
-  EWPW (ShallowTryLSV e l h r) @E <| ρ' |> {{ Φ' }}.
+Lemma ewpw_shandler E (op : operation) m σ ρ ρ' e (h r : val) Φ Φ' :
+  EWPW e @ E <| (op, σ) ·: ρ |> {{ Φ }} -∗
+  shandler_spec E op σ ρ m Φ h r ρ' Φ' -∗
+  EWPW (SHandlerV e op h r) @E <| ρ' |> {{ Φ' }}.
 Proof.
-  iIntros "He H". rewrite /ShallowTryLSV /shallow_try_ls /ewpw. 
-  iLöb as "IH" forall (e). ewp_pure_steps.
+  iIntros "He H". rewrite /SHandlerV /ewpw. 
+  iLöb as "IH" forall (e). rewrite {2} /shandler. ewp_pure_steps.
   iApply (ewp_try_with_mode with "He").
-  rewrite /shallow_handler_ls.
+  rewrite /shandler_spec.
   iDestruct "H" as "(#Hle & %HOS & Hbr)". 
   iSplit; last iSplit.
   - rewrite {2} bi.intuitionistically_if_elim. iDestruct "Hbr" as "[$ _]".
   - iIntros (v k) "Hρ".
     ewp_pure_steps. 
-    iDestruct "Hρ" as "(%Φ'' & (%v' & %l' & %s' & %σ' & %Heq' & Hlookup' & Hσ') & HPost)".
-    inv Heq'. destruct (decide (l = l' ∧ s' = 0)) as [[-> ->]|Hneg].
+    iDestruct "Hρ" as "(%Φ'' & (%v' & %op' & %s' & %σ' & %Heq' & Hlookup' & Hσ') & HPost)".
+    inv Heq'. destruct (decide (op = op' ∧ s' = 0)) as [[-> ->]|Hneg].
     + ewp_pure_steps'.
       rewrite {2} bi.intuitionistically_if_elim. iDestruct "Hbr" as "[_ H]".
       iApply "H". iExists Φ''. 
@@ -462,15 +462,15 @@ Proof.
       ewp_pure_steps. iApply ewp_do_os. iExists Φ''. simpl. 
       rewrite filter_os_lookup lookup_insert_ne; last (intros H'; inv H'; tauto).
       iSplitR "HPost Hbr".
-      { iExists v', l', s', σ'. iFrame "#∗". iSplit; first done. 
+      { iExists v', op', s', σ'. iFrame "#∗". iSplit; first done. 
         rewrite filter_os_lookup. iFrame. }
       iIntros (w) "HΦ''". do 5 ewp_value_or_step.
       iApply ("IH" with "[HΦ'' HPost] [Hbr]"); first by iApply "HPost".
       by iFrame "#∗".
   - iIntros (v k) "Hρ".
     ewp_pure_steps. 
-    iDestruct "Hρ" as "(%Φ'' & (%v' & %l' & %s' & %σ' & %Heq' & #Hlookup' & Hσ') & #HPost)".
-    inv Heq'. destruct (decide (l = l' ∧ s' = 0)) as [[-> ->]|Hneg].
+    iDestruct "Hρ" as "(%Φ'' & (%v' & %op' & %s' & %σ' & %Heq' & #Hlookup' & Hσ') & #HPost)".
+    inv Heq'. destruct (decide (op = op' ∧ s' = 0)) as [[-> ->]|Hneg].
     + ewp_pure_steps'.
       rewrite {2} bi.intuitionistically_if_elim. iDestruct "Hbr" as "[_ H]".
       iApply "H". iExists Φ''. 
@@ -484,30 +484,30 @@ Proof.
       ewp_pure_steps. rewrite lookup_insert_ne; last (intros H'; inv H'; tauto).
       iApply ewp_do_ms. destruct m; simpl.
       * specialize (HOS eq_refl).
-        iDestruct (os_row_mono_prot _ l' s' σ' with "Hlookup'") as "Hmono".
-        iAssert (shallow_handler_ls E l σ _ OS Φ h r ρ' Φ') with "[Hbr]" as "H".
-        { rewrite /shallow_handler_ls. simpl. by iFrame "#∗". }
-        iExists (λ v, Φ'' v ∗ shallow_handler_ls E l σ ρ OS Φ h r ρ' Φ')%I.
+        iDestruct (os_row_mono_prot _ op' s' σ' with "Hlookup'") as "Hmono".
+        iAssert (shandler_spec E op σ _ OS Φ h r ρ' Φ') with "[Hbr]" as "H".
+        { rewrite /shandler_spec. simpl. by iFrame "#∗". }
+        iExists (λ v, Φ'' v ∗ shandler_spec E op σ ρ OS Φ h r ρ' Φ')%I.
         iSplitL; [|iIntros "!# %w [HΦ'' H]"; do 5 ewp_value_or_step; 
                    iSpecialize ("HPost" with "HΦ''"); iApply ("IH" with "HPost H")].
-        iExists v', l', s', σ'. iFrame "#∗".
+        iExists v', op', s', σ'. iFrame "#∗".
         iSplit; [done|]. iApply ("Hmono" with "[H] Hσ'"). iIntros (w) "$ //".
       * iDestruct "Hbr" as "#Hbr".
         iExists Φ''. iSplitL "Hσ'".
-        { iExists v', l', s', σ'. by iFrame "#∗". }
+        { iExists v', op', s', σ'. by iFrame "#∗". }
         iIntros (w) "!# HΦ''". do 5 ewp_value_or_step.
         iApply ("IH" with "[HΦ'' HPost] [Hbr]"); first by iApply "HPost".
         by iFrame "#∗".
 Qed.
 
-Notation deep_handler_ls_type Σ :=
-  (coPset -d> label-d> sem_sig Σ -d> sem_row Σ -d> mode -d> (val -d> iPropO Σ) 
+Notation handler_spec_type Σ :=
+  (coPset -d> sem_sig Σ -d> sem_row Σ -d> mode -d> (val -d> iPropO Σ) 
           -d> expr -d> expr
           -d> sem_row Σ -d> (val -d> iPropO Σ) -d> iPropO Σ) (only parsing).
 
-Definition deep_handler_ls_pre `{irisGS eff_lang Σ} : 
-  deep_handler_ls_type Σ → deep_handler_ls_type Σ := (
-  λ deep_handler_ls E l σ ρ m Φ h r ρ' Φ',
+Definition handler_spec_pre `{irisGS eff_lang Σ} : 
+  handler_spec_type Σ → handler_spec_type Σ := (
+  λ handler_spec E σ ρ m Φ h r ρ' Φ',
   (* Subsumption on row *)
   (ρ ≤R ρ') ∗
 
@@ -524,50 +524,44 @@ Definition deep_handler_ls_pre `{irisGS eff_lang Σ} :
   (∀ (v k : val),
      iEff_car (upcl σ.1 σ.2) v (λ w, 
         ∀ ρ'' Φ'', 
-          ▷ deep_handler_ls E l σ ρ m Φ h r ρ'' Φ'' -∗
+          ▷ handler_spec E σ ρ m Φ h r ρ'' Φ'' -∗
           EWPW k w @ E <| ρ'' |> {{ Φ'' }}
      ) -∗
        EWPW h v k @ E <| ρ' |> {{ Φ' }}))
   )%I.
 
-(*            osrow *)
-(*         | OS  | MS *)   
-(*    ------------------- *)
-(*    | OS | ros | rms *)
-(* m  | MS | rms | rms *)
-
-Local Instance deep_handler_ls_pre_contractive `{irisGS eff_lang Σ} : Contractive deep_handler_ls_pre.
+Local Instance handler_spec_pre_contractive `{irisGS eff_lang Σ} : Contractive handler_spec_pre.
 Proof.
-  rewrite /deep_handler_ls_pre => n deep deep' Hne E l σ ρ m Φ h r ρ' Φ'.
+  rewrite /handler_spec_pre => n deep deep' Hne E σ ρ m Φ h r ρ' Φ'.
   repeat (f_contractive || f_equiv). intros ?; simpl.
   repeat (f_contractive || f_equiv); apply Hne.
 Qed.
-Definition deep_handler_ls `{irisGS eff_lang Σ} := fixpoint deep_handler_ls_pre.
-Arguments deep_handler_ls _ _%V _%S _%R _%I _%E _%E _%R _%I.
+Definition handler_spec `{irisGS eff_lang Σ} := fixpoint handler_spec_pre.
+Arguments handler_spec _ _%S _%R _%I _%E _%E _%R _%I.
 
-Global Lemma deep_handler_ls_unfold `{irisGS eff_lang Σ} E l σ ρ m Φ h r ρ' Φ' :
-  deep_handler_ls E l σ ρ m Φ h r ρ' Φ' ⊣⊢
-    deep_handler_ls_pre deep_handler_ls E l σ ρ m Φ h r ρ' Φ'.
+Global Lemma handler_spec_unfold `{irisGS eff_lang Σ} E σ ρ m Φ h r ρ' Φ' :
+  handler_spec E σ ρ m Φ h r ρ' Φ' ⊣⊢
+    handler_spec_pre handler_spec E σ ρ m Φ h r ρ' Φ'.
 Proof.
-  by apply (fixpoint_unfold deep_handler_ls_pre).
+  by apply (fixpoint_unfold handler_spec_pre).
 Qed.
 
-Lemma ewpw_deep_try_ls E (l : label) m σ ρ ρ' e (h r : val) Φ Φ' :
-  EWPW e @ E <| (l, σ) ·: ρ |> {{ Φ }} -∗
-  deep_handler_ls E l σ ρ m Φ h r ρ' Φ' -∗
-  EWPW (DeepTryLSV e l h r) @E <| ρ' |> {{ Φ' }}.
+Lemma ewpw_handler E (op : operation) m σ ρ ρ' e (h r : val) Φ Φ' :
+  EWPW e @ E <| (op, σ) ·: ρ |> {{ Φ }} -∗
+  handler_spec E σ ρ m Φ h r ρ' Φ' -∗
+  EWPW (HandlerV e op h r) @E <| ρ' |> {{ Φ' }}.
 Proof.
-  iIntros "He H". rewrite /DeepTryLSV /deep_try_ls /ewpw. 
+  iIntros "He H". rewrite /HandlerV /handler /ewpw. 
   ewp_pure_steps.
   iApply (ewp_deep_try_with_mode with "He").
-  iLöb as "IH" forall (ρ' Φ'). rewrite deep_handler_ls_unfold.
+  iLöb as "IH" forall (ρ' Φ'). rewrite handler_spec_unfold.
   iDestruct "H" as "(#Hle & %HOS & Hbr)". 
   rewrite deep_handler_mode_unfold /deep_handler_mode_pre.
   iSplit; last iSplit.
   - rewrite bi.intuitionistically_if_elim. iDestruct "Hbr" as "[$ _]".
   - iIntros (v k) "Hρ". ewp_pure_steps. 
-    iDestruct "Hρ" as "(%Φ'' & (%v' & %l' & %s' & %σ' & %Heq' & Hlookup' & Hσ') & HPost)".
-    inv Heq'. destruct (decide (l = l' ∧ s' = 0)) as [[-> ->]|Hneg].
+    iDestruct "Hρ" as "(%Φ'' & (%v' & %op' & %s' & %σ' & %Heq' & Hlookup' & Hσ') & HPost)".
+    inv Heq'. destruct (decide (op = op' ∧ s' = 0)) as [[-> ->]|Hneg].
     + ewp_pure_steps'.
       rewrite bi.intuitionistically_if_elim. iDestruct "Hbr" as "[_ H]".
       iApply "H". iExists Φ''. 
@@ -586,12 +580,12 @@ Proof.
       ewp_pure_steps. iApply ewp_do_os. iExists Φ''. simpl. 
       rewrite filter_os_lookup lookup_insert_ne //; last (intros H'; inv H'; tauto).
       iSplitR "HPost Hbr".
-      { iExists v', l', s', σ'. iFrame "#∗". iSplit; first done. rewrite filter_os_lookup //. }
+      { iExists v', op', s', σ'. iFrame "#∗". iSplit; first done. rewrite filter_os_lookup //. }
       iIntros (w) "HΦ''". iApply ("HPost" with "HΦ''"). iNext. iApply ("IH" with "[Hbr]").
-      destruct m; rewrite deep_handler_ls_unfold /deep_handler_ls_pre; iFrame "#∗"; eauto.
+      destruct m; rewrite handler_spec_unfold /handler_spec_pre; iFrame "#∗"; eauto.
   - iIntros (v k) "Hρ". ewp_pure_steps. 
-    iDestruct "Hρ" as "(%Φ'' & (%v' & %l' & %s' & %σ' & %Heq' & #Hlookup' & Hσ') & #HPost)".
-    inv Heq'. destruct (decide (l = l' ∧ s' = 0)) as [[-> ->]|Hneg].
+    iDestruct "Hρ" as "(%Φ'' & (%v' & %op' & %s' & %σ' & %Heq' & #Hlookup' & Hσ') & #HPost)".
+    inv Heq'. destruct (decide (op = op' ∧ s' = 0)) as [[-> ->]|Hneg].
     + ewp_pure_steps'.
       rewrite bi.intuitionistically_if_elim. iDestruct "Hbr" as "[_ H]".
       iApply "H". iExists Φ''. 
@@ -606,34 +600,34 @@ Proof.
       ewp_pure_steps. rewrite lookup_insert_ne; last (intros H'; inv H'; tauto).
       iApply ewp_do_ms. destruct m; simpl.
       * specialize (HOS eq_refl).
-        iDestruct (os_row_mono_prot _ l' s' σ' with "Hlookup'") as "Hmono".
-        iAssert (deep_handler_ls E l σ ρ OS Φ h r ρ' Φ') with "[Hbr]" as "H".
-        { rewrite deep_handler_ls_unfold /deep_handler_ls_pre. simpl. by iFrame "#∗". }
-        iExists (λ v, Φ'' v ∗ deep_handler_ls E l σ ρ OS Φ h r ρ' Φ')%I.
+        iDestruct (os_row_mono_prot _ op' s' σ' with "Hlookup'") as "Hmono".
+        iAssert (handler_spec E σ ρ OS Φ h r ρ' Φ') with "[Hbr]" as "H".
+        { rewrite handler_spec_unfold /handler_spec_pre. simpl. by iFrame "#∗". }
+        iExists (λ v, Φ'' v ∗ handler_spec E σ ρ OS Φ h r ρ' Φ')%I.
         iSplitL; [|iIntros "!# %w [HΦ'' Hdeep]"; iApply ("HPost" with "HΦ''"); iNext; by iApply "IH"].
-        iExists v', l', s', σ'. iFrame "#∗". iSplit; [done|]. 
+        iExists v', op', s', σ'. iFrame "#∗". iSplit; [done|]. 
         iApply ("Hmono" with "[H] Hσ'"). iIntros (w) "$ //".
       * iDestruct "Hbr" as "#Hbr".
         iExists Φ''. iSplitL "Hσ'".
-        { iExists v', l', s', σ'. by iFrame "#∗". }
+        { iExists v', op', s', σ'. by iFrame "#∗". }
         iIntros (w) "!# HΦ''". iApply ("HPost" with "HΦ''").
         iNext. iApply "IH".
-        rewrite deep_handler_ls_unfold /deep_handler_ls_pre. simpl. by iFrame "#∗". 
+        rewrite handler_spec_unfold /handler_spec_pre. simpl. by iFrame "#∗". 
 Qed.
 
-Notation deep_handler_ls_2_type Σ :=
-  (coPset -d> label -d> sem_sig Σ -d> label -d> sem_sig Σ -d> sem_row Σ -d> mode -d> (val -d> iPropO Σ) 
+Notation handler2_spec_type Σ :=
+  (coPset -d> operation -d> sem_sig Σ -d> operation -d> sem_sig Σ -d> sem_row Σ -d> mode -d> (val -d> iPropO Σ) 
           -d> expr  -d> expr -d> expr
           -d> sem_row Σ -d> (val -d> iPropO Σ) -d> iPropO Σ) (only parsing).
 
-Definition deep_handler_ls_2_pre `{irisGS eff_lang Σ} : 
-  deep_handler_ls_2_type Σ → deep_handler_ls_2_type Σ := (
-  λ deep_handler_ls_2 E l1 σ1 l2 σ2 ρ m Φ h1 h2 r ρ' Φ',
+Definition handler2_spec_pre `{irisGS eff_lang Σ} : 
+  handler2_spec_type Σ → handler2_spec_type Σ := (
+  λ handler2_spec E op1 σ1 op2 σ2 ρ m Φ h1 h2 r ρ' Φ',
 
   (* Subsumption on row *)
   (ρ ≤R ρ') ∗
 
-  ⌜ l1 ≠ l2 ⌝ ∗
+  ⌜ op1 ≠ op2 ⌝ ∗
 
   (* One-Shot Row *)
   (⌜ m = OS → OSRow ρ ⌝) ∗
@@ -648,7 +642,7 @@ Definition deep_handler_ls_2_pre `{irisGS eff_lang Σ} :
   (∀ (v k : val),
      iEff_car (upcl σ1.1 σ1.2) v (λ w, 
         ∀ ρ'' Φ'', 
-          ▷ deep_handler_ls_2 E l1 σ1 l2 σ2 ρ m Φ h1 h2 r ρ'' Φ'' -∗
+          ▷ handler2_spec E op1 σ1 op2 σ2 ρ m Φ h1 h2 r ρ'' Φ'' -∗
           EWPW k w @ E <| ρ'' |> {{ Φ'' }}
      ) -∗
        EWPW h1 v k @ E <| ρ' |> {{ Φ' }}) ∧
@@ -657,45 +651,45 @@ Definition deep_handler_ls_2_pre `{irisGS eff_lang Σ} :
   (∀ (v k : val),
      iEff_car (upcl σ2.1 σ2.2) v (λ w, 
         ∀ ρ'' Φ'', 
-          ▷ deep_handler_ls_2 E l1 σ1 l2 σ2 ρ m Φ h1 h2 r ρ'' Φ'' -∗
+          ▷ handler2_spec E op1 σ1 op2 σ2 ρ m Φ h1 h2 r ρ'' Φ'' -∗
           EWPW k w @ E <| ρ'' |> {{ Φ'' }}
      ) -∗
        EWPW h2 v k @ E <| ρ' |> {{ Φ' }})
   ))%I.
 
-Local Instance deep_handler_ls_2_pre_contractive `{irisGS eff_lang Σ} : Contractive deep_handler_ls_2_pre.
+Local Instance handler2_spec_pre_contractive `{irisGS eff_lang Σ} : Contractive handler2_spec_pre.
 Proof.
-  rewrite /deep_handler_ls_2_pre => n deep deep' Hne E l1 σ1 l2 σ2 ρ m Φ h1 h2 r ρ' Φ'.
+  rewrite /handler2_spec_pre => n deep deep' Hne E l1 σ1 l2 σ2 ρ m Φ h1 h2 r ρ' Φ'.
   repeat (f_contractive || f_equiv). intros ?; simpl.
   repeat (f_contractive || f_equiv); apply Hne.
   intros ?. repeat (f_contractive || f_equiv); apply Hne.
 Qed.
-Definition deep_handler_ls_2 `{irisGS eff_lang Σ} := fixpoint deep_handler_ls_2_pre.
-Arguments deep_handler_ls_2 _ _%V _%S _%V _%S _%R _%I _%E _%E _%E _%R _%I.
+Definition handler2_spec `{irisGS eff_lang Σ} := fixpoint handler2_spec_pre.
+Arguments handler2_spec _ _%V _%S _%V _%S _%R _%I _%E _%E _%E _%R _%I.
 
-Global Lemma deep_handler_ls_2_unfold `{irisGS eff_lang Σ} E l1 σ1 l2 σ2 ρ m Φ h1 h2 r ρ' Φ' :
-  deep_handler_ls_2 E l1 σ1 l2 σ2 ρ m Φ h1 h2 r ρ' Φ' ⊣⊢
-    deep_handler_ls_2_pre deep_handler_ls_2 E l1 σ1 l2 σ2 ρ m Φ h1 h2 r ρ' Φ'.
+Global Lemma handler2_spec_unfold `{irisGS eff_lang Σ} E op1 σ1 op2 σ2 ρ m Φ h1 h2 r ρ' Φ' :
+  handler2_spec E op1 σ1 op2 σ2 ρ m Φ h1 h2 r ρ' Φ' ⊣⊢
+    handler2_spec_pre handler2_spec E op1 σ1 op2 σ2 ρ m Φ h1 h2 r ρ' Φ'.
 Proof.
-  by apply (fixpoint_unfold deep_handler_ls_2_pre).
+  by apply (fixpoint_unfold handler2_spec_pre).
 Qed.
 
-Lemma ewpw_deep_try_ls_2 E (l1 l2 : label) m σ1 σ2 ρ ρ' e (h1 h2 r : val) Φ Φ' :
-  EWPW e @ E <| (l1, σ1) ·: (l2, σ2) ·: ρ |> {{ Φ }} -∗
-  deep_handler_ls_2 E l1 σ1 l2 σ2 ρ m Φ h1 h2 r ρ' Φ' -∗
-  EWPW (DeepTryLS2V e l1 l2 h1 h2 r) @E <| ρ' |> {{ Φ' }}.
+Lemma ewpw_handler2 E (op1 op2 : operation) m σ1 σ2 ρ ρ' e (h1 h2 r : val) Φ Φ' :
+  EWPW e @ E <| (op1, σ1) ·: (op2, σ2) ·: ρ |> {{ Φ }} -∗
+  handler2_spec E op1 σ1 op2 σ2 ρ m Φ h1 h2 r ρ' Φ' -∗
+  EWPW (Handler2V e op1 op2 h1 h2 r) @E <| ρ' |> {{ Φ' }}.
 Proof.
-  iIntros "He H". rewrite /DeepTryLS2V /deep_try_ls_2 /ewpw. 
+  iIntros "He H". rewrite /Handler2V /handler2 /ewpw. 
   ewp_pure_steps.
   iApply (ewp_deep_try_with_mode with "He").
-  iLöb as "IH" forall (ρ' Φ'). rewrite deep_handler_ls_2_unfold.
+  iLöb as "IH" forall (ρ' Φ'). rewrite handler2_spec_unfold.
   iDestruct "H" as "(#Hle & %Hneq & %HOS & Hbr)". 
   rewrite deep_handler_mode_unfold /deep_handler_mode_pre.
   iSplit; last iSplit.
   - rewrite bi.intuitionistically_if_elim. iDestruct "Hbr" as "[$ _]".
   - iIntros (v k) "Hρ". ewp_pure_steps. 
-    iDestruct "Hρ" as "(%Φ'' & (%v' & %l' & %s' & %σ' & %Heq' & Hlookup' & Hσ') & HPost)".
-    inv Heq'. destruct (decide (l1 = l' ∧ s' = 0)) as [[-> ->]|Hneg].
+    iDestruct "Hρ" as "(%Φ'' & (%v' & %op' & %s' & %σ' & %Heq' & Hlookup' & Hσ') & HPost)".
+    inv Heq'. destruct (decide (op1 = op' ∧ s' = 0)) as [[-> ->]|Hneg].
     + ewp_pure_steps'.
       rewrite bi.intuitionistically_if_elim. iDestruct "Hbr" as "[_ H]".
       iApply "H". iExists Φ''. 
@@ -707,7 +701,7 @@ Proof.
       iRewrite "HσOS". simpl. iIntros (w) "HΦ''". 
       iIntros (ρ'' Φ''') "Hdeep". iApply ("HPost" with "HΦ''").
       iNext. iApply ("IH" with "Hdeep"). 
-    + destruct (decide (l2 = l' ∧ s' = 0)) as [[-> ->]|Hneg'].
+    + destruct (decide (op2 = op' ∧ s' = 0)) as [[-> ->]|Hneg'].
       * ewp_pure_steps'.
         rewrite bi.intuitionistically_if_elim. iDestruct "Hbr" as "[_ [_ H]]".
         iApply "H". iExists Φ''. 
@@ -728,14 +722,14 @@ Proof.
         ewp_pure_steps. iApply ewp_do_os. iExists Φ''. simpl. 
         rewrite filter_os_lookup lookup_insert_ne //; last (intros H'; inv H'; tauto).
         iSplitR "HPost Hbr".
-        { iExists v', l', s', σ'. iFrame "#∗". iSplit; first done. rewrite filter_os_lookup //. 
+        { iExists v', op', s', σ'. iFrame "#∗". iSplit; first done. rewrite filter_os_lookup //. 
           rewrite /sem_row_cons row_tun_ins_eq_ne // lookup_insert_ne; first iFrame.
           intros H. inv H; apply Hneg'; eauto. }
       iIntros (w) "HΦ''". iApply ("HPost" with "HΦ''"). iNext. iApply ("IH" with "[Hbr]").
-      destruct m; rewrite deep_handler_ls_2_unfold /deep_handler_ls_2_pre; iFrame "#∗"; eauto.
+      destruct m; rewrite handler2_spec_unfold /handler2_spec_pre; iFrame "#∗"; eauto.
   - iIntros (v k) "Hρ". ewp_pure_steps. 
-    iDestruct "Hρ" as "(%Φ'' & (%v' & %l' & %s' & %σ' & %Heq' & #Hlookup' & Hσ') & #HPost)".
-    inv Heq'. destruct (decide (l1 = l' ∧ s' = 0)) as [[-> ->]|Hneg].
+    iDestruct "Hρ" as "(%Φ'' & (%v' & %op' & %s' & %σ' & %Heq' & #Hlookup' & Hσ') & #HPost)".
+    inv Heq'. destruct (decide (op1 = op' ∧ s' = 0)) as [[-> ->]|Hneg].
     + ewp_pure_steps'.
       rewrite bi.intuitionistically_if_elim. iDestruct "Hbr" as "[_ H]".
       iApply "H". iExists Φ''. 
@@ -743,7 +737,7 @@ Proof.
       iRewrite - ("Hlookup'" $! v' Φ'') in "Hσ'". iFrame.
       destruct σ1.1; simpl; last iIntros "!#"; 
       iIntros (w) "HΦ'' % %Φ''' Hdeep"; iApply ("HPost" with "HΦ''"); iNext; by iApply "IH".
-    + destruct (decide (l2 = l' ∧ s' = 0)) as [[-> ->]|Hneg'].
+    + destruct (decide (op2 = op' ∧ s' = 0)) as [[-> ->]|Hneg'].
       * ewp_pure_steps'.
         rewrite bi.intuitionistically_if_elim. iDestruct "Hbr" as "[_ [_ H]]". 
         iApply "H". iExists Φ''. 
@@ -763,19 +757,19 @@ Proof.
         2: { intros H. inv H; apply Hneg'; eauto. }
         iApply ewp_do_ms. destruct m; simpl.
         ** specialize (HOS eq_refl).
-          iDestruct (os_row_mono_prot _ l' s' σ' with "Hlookup'") as "Hmono".
-          iAssert (deep_handler_ls_2 E l1 σ1 l2 σ2 ρ OS Φ h1 h2 r ρ' Φ') with "[Hbr]" as "H".
-          { rewrite deep_handler_ls_2_unfold /deep_handler_ls_2_pre. simpl. by iFrame "#∗". }
-          iExists (λ v, Φ'' v ∗ deep_handler_ls_2 E l1 σ1 l2 σ2 ρ OS Φ h1 h2 r ρ' Φ')%I.
+          iDestruct (os_row_mono_prot _ op' s' σ' with "Hlookup'") as "Hmono".
+          iAssert (handler2_spec E op1 σ1 op2 σ2 ρ OS Φ h1 h2 r ρ' Φ') with "[Hbr]" as "H".
+          { rewrite handler2_spec_unfold /handler2_spec_pre. simpl. by iFrame "#∗". }
+          iExists (λ v, Φ'' v ∗ handler2_spec E op1 σ1 op2 σ2 ρ OS Φ h1 h2 r ρ' Φ')%I.
           iSplitL; [|iIntros "!# %w [HΦ'' Hdeep]"; iApply ("HPost" with "HΦ''"); iNext; by iApply "IH"].
-          iExists v', l', s', σ'. iFrame "#∗". iSplit; [done|]. 
+          iExists v', op', s', σ'. iFrame "#∗". iSplit; [done|]. 
           iApply ("Hmono" with "[H] Hσ'"). iIntros (w) "$ //".
         ** iDestruct "Hbr" as "#Hbr".
            iExists Φ''. iSplitL "Hσ'".
-           { iExists v', l', s', σ'. by iFrame "#∗". }
+           { iExists v', op', s', σ'. by iFrame "#∗". }
         iIntros (w) "!# HΦ''". iApply ("HPost" with "HΦ''").
         iNext. iApply "IH".
-        rewrite deep_handler_ls_2_unfold /deep_handler_ls_2_pre. simpl. by iFrame "#∗". 
+        rewrite handler2_spec_unfold /handler2_spec_pre. simpl. by iFrame "#∗". 
 Qed.
      
 End reasoning.
