theories/case_studies/state.v
@@ -25,8 +25,8 @@ From haffel.logic Require Import sem_operators.
 From haffel.logic Require Import compatibility.
 From haffel.logic Require Import tactics.
 
-Definition get : val := (λ: <>, performₘ: (effect "get", #()))%V.
-Definition put : val := (λ: "s", (performₘ: (effect "put", "s")))%V.
+Definition get : val := (λ: <>, performₘ: "get" #())%V.
+Definition put : val := (λ: "s", performₘ: "put" "s")%V.
 
 Definition fact : val :=
   (rec: "fact" "n" := if: #1 < "n" then put (get #() * "n");; "fact" ("n" - #1)
@@ -34,26 +34,26 @@ Definition fact : val :=
 
 Definition fact_ref : val :=
   (λ: "n", let: "store" := ref #1 in
-      deep-try-ls2: (fact "n") with
-          effect "get" => (λ: "x" "k", "k" (Load "store"))
-        | effect "put" => (λ: "x" "k", "store" <- "x" ;; "k" #())
-        | return (λ: "x", Load "store")
+      handle2: (fact "n") by
+          "get" => (λ: "x" "k", "k" (Load "store"))
+        | "put" => (λ: "x" "k", "store" <- "x" ;; "k" #())
+        |  ret  => (λ: "x", Load "store")
       end)%V.
 
 Definition fact_st : val :=
   (λ: "n", 
-    (deep-try-ls2: (fact "n") with
-        effect "get" => (λ: "x" "k", (λ: "s", "k" "s" "s"))
-      | effect "put" => (λ: "x" "k", (λ: <>, "k" #() "x"))
-      | return (λ: "x", (λ: "y", "y"))
+    (handle2: (fact "n") by
+        "get" => (λ: "x" "k", (λ: "s", "k" "s" "s"))
+      | "put" => (λ: "x" "k", (λ: <>, "k" #() "x"))
+      |  ret  => (λ: "x", (λ: "y", "y"))
       end #1))%V.
 
 Section typing.
 
   Context `{!heapGS Σ}.
 
-  Definition putsig : label * sem_sig Σ := ("put", ∀S: _, ℤ ⇒ () | MS)%S.  
-  Definition getsig : label * sem_sig Σ := ("get", ∀S: _, () ⇒ ℤ | MS)%S.
+  Definition putsig : operation * sem_sig Σ := ("put", ∀S: _, ℤ ⇒ () | MS)%S.  
+  Definition getsig : operation * sem_sig Σ := ("get", ∀S: _, () ⇒ ℤ | MS)%S.
   Definition st : sem_row Σ := (putsig ·: getsig ·: ⟨⟩)%R.
 
   Lemma get_typed :
@@ -114,7 +114,7 @@ Section typing.
     simpl. iApply (sem_typed_let _ _ _ _ [("n", ℤ)]); solve_sidecond. 
     { iApply sem_typed_alloc_cpy. iApply sem_typed_int. }
     iApply sem_typed_swap_second. rewrite app_singletons. 
-    iApply (sem_typed_deep_try_2_ms "get" "put" (λ _, ()) (λ _, ℤ) (λ _, ℤ) (λ _, ()) () ℤ ⊥ _ _ [] with "[] [] []"); solve_sidecond.
+    iApply (sem_typed_handler2_ms "get" "put" (λ _, ()) (λ _, ℤ) (λ _, ℤ) (λ _, ()) () ℤ ⊥ _ _ [] with "[] [] []"); solve_sidecond.
     { iApply row_le_refl. }
     - iApply sem_typed_sub_row; first by iApply row_le_swap_second.
       iApply (sem_typed_app_ms ℤ); solve_copy; last iApply sem_typed_var'.
@@ -142,7 +142,7 @@ Section typing.
     iIntros. iApply sem_typed_closure; solve_sidecond.
     simpl. iApply (sem_typed_app_ms ℤ); solve_copy; last iApply sem_typed_int.
     rewrite - {1} (app_nil_r [("n", ℤ)]).
-    iApply (sem_typed_deep_try_2_ms "get" "put" (λ _, ()) (λ _, ℤ) (λ _, ℤ) (λ _, ()) () _ _ _ _ []); solve_sidecond.
+    iApply (sem_typed_handler2_ms "get" "put" (λ _, ()) (λ _, ℤ) (λ _, ℤ) (λ _, ()) () _ _ _ _ []); solve_sidecond.
     { iApply row_le_refl. }
     - iApply sem_typed_sub_row; first by iApply row_le_swap_second.
       iApply (sem_typed_app_ms ℤ); solve_copy; last iApply sem_typed_var'.
